Alternative VariableNoUpd; better ind_for

Launchbury/RemoveTaggedIndirection.thy
@@ -2,32 +2,6 @@ theory RemoveTaggedIndirection
 imports LaunchburyCombinedTagged Indirections "Nominal-Utils"
 begin
 
-consts resolveStack :: "var list \<Rightarrow> indirections \<Rightarrow> var list"(infixl "\<ominus>\<^sub>S" 60)
-
-lemma resolveStack_Cons_not[simp]: "x \<notin> heapVars is \<Longrightarrow> (x # S) \<ominus>\<^sub>S is = x # (S \<ominus>\<^sub>S is)"
-  sorry
-
-lemma resolveStack_eqvt[eqvt]: "\<pi> \<bullet> (S \<ominus>\<^sub>S is) = (\<pi> \<bullet> S) \<ominus>\<^sub>S (\<pi> \<bullet> is)"
-  sorry
-
-lemma resolveStack_set[simp]: "x \<notin> heapVars is \<Longrightarrow> x \<in> set (S \<ominus>\<^sub>S is) \<longleftrightarrow> x \<in> set S"
-  sorry
-
-lemma resolveStack_fresh_noop[simp]: "atom z \<sharp> S \<Longrightarrow> (S \<ominus>\<^sub>S (z, y) # is) = (S \<ominus>\<^sub>S is)"
-  sorry
-
-lemma resolveStack_ConsCons[simp]:
-  "(x, y) \<in> set is \<Longrightarrow> y # x # S \<ominus>\<^sub>S is = x # S \<ominus>\<^sub>S is" sorry
-
-definition ind_for :: "indirections \<Rightarrow> heap \<Rightarrow> bool" where
-  "ind_for is \<Gamma> = (\<forall> (x,y) \<in> set is. (x, Var y) \<in> set \<Gamma>)"
-
-lemma ind_for_heapVars_subset:
-  "ind_for is \<Gamma> \<Longrightarrow> heapVars is \<subseteq> heapVars \<Gamma>"
-  unfolding ind_for_def
-  apply (auto simp add: heapVars_def)
-  by (metis (lifting) fst_conv imageI splitD)
-
 nominal_primrec isVar :: "exp \<Rightarrow> bool" where
   "isVar (Var x) = True" |
   "isVar (Lam [x]. e) = False" |
@@ -41,37 +15,113 @@ nominal_primrec isVar :: "exp \<Rightarrow> bool" where
   done
 termination (eqvt) by lexicographic_order
 
-lemma non_var_not_ind:
-  "distinctVars \<Gamma> \<Longrightarrow> ind_for is \<Gamma> \<Longrightarrow> (x,e) \<in> set \<Gamma> \<Longrightarrow> x \<in> heapVars is \<Longrightarrow> isVar e"
-  unfolding heapVars_def ind_for_def
-  by (auto dest: distinctVarsE)
+nominal_primrec isLam :: "exp \<Rightarrow> bool" where
+  "isLam (Var x) = False" |
+  "isLam (Lam [x]. e) = True" |
+  "isLam (App e x) = False" |
+  "isLam (Let as e) = False"
+  unfolding isLam_graph_aux_def eqvt_def
+  apply simp
+  apply simp
+  apply (metis exp_assn.exhaust(1))
+  apply auto
+  done
+termination (eqvt) by lexicographic_order
 
-lemma ind_for_Cons[simp]: "\<not> isVar e \<Longrightarrow> ind_for is ((x,e)#\<Gamma>) \<longleftrightarrow> ind_for is \<Gamma>"
-  unfolding ind_for_def by auto
 
+fun remdups' :: "'a list \<Rightarrow> 'a list" where
+  "remdups' [] = []" |
+  "remdups' (x#xs) = x # removeAll x (remdups' xs)"
+
+definition resolveStack :: "var list \<Rightarrow> indirections \<Rightarrow> var list"(infixl "\<ominus>\<^sub>S" 60)
+  where "resolveStack xs is = remdups' (xs \<ominus> is)"
+
+lemma resolveStack_Cons[simp]: "(x # S) \<ominus>\<^sub>S is = (x \<ominus> is) # (removeAll (x \<ominus> is) (S \<ominus>\<^sub>S is))"
+  unfolding resolveStack_def by simp
+
+lemma resolveStack_eqvt[eqvt]: "\<pi> \<bullet> (S \<ominus>\<^sub>S is) = (\<pi> \<bullet> S) \<ominus>\<^sub>S (\<pi> \<bullet> is)"
+  sorry
+
+(*
+lemma resolveStack_set[simp]: "x \<notin> heapVars is \<Longrightarrow> x \<in> set (S \<ominus>\<^sub>S is) \<longleftrightarrow> x \<in> set S"
+  sorry
+*)
+
+lemma resolveStack_fresh_noop[simp]: "atom z \<sharp> S \<Longrightarrow> (S \<ominus>\<^sub>S (z, y) # is) = (S \<ominus>\<^sub>S is)"
+  unfolding resolveStack_def by (induction "is" arbitrary: S) auto
+
+lemma valid_ind_different: "valid_ind is \<Longrightarrow> (x,y) \<in> set is \<Longrightarrow> x \<noteq> y"
+  by (induct  "is" rule: valid_ind.induct) (auto simp add: fresh_Pair)
+
+lemma resolve_var_modifies: "valid_ind is \<Longrightarrow> x \<in> heapVars is \<Longrightarrow> x \<noteq> x \<ominus> is" 
+  sorry
+
+lemma resolve_var_same_image[dest]: "valid_ind is \<Longrightarrow> (x,y) \<in> set is \<Longrightarrow> x \<ominus> is = y \<ominus> is"
+  apply (induct  "is" rule: valid_ind.induct)
+  apply (auto simp add: fresh_Pair)
+  apply (metis heapVars_from_set heapVars_not_fresh)
+  apply (metis fresh_heap_expr not_self_fresh)
+  done
+
+lemma resolveStack_ConsCons[simp]:
+  "valid_ind is \<Longrightarrow> (x, y) \<in> set is \<Longrightarrow> y # x # S \<ominus>\<^sub>S is = (y \<ominus> is) # (removeAll (y \<ominus> is) (S \<ominus>\<^sub>S is))"
+  unfolding resolveStack_def by auto
+
+definition ind_for :: "indirections \<Rightarrow> heap \<Rightarrow> bool" where
+  "ind_for is \<Gamma> = (\<forall> (x,y) \<in> set is. (x \<in> heapVars \<Gamma> \<and> ((map_of \<Gamma> x) = Some (Var y) \<or> (isLam (the (map_of \<Gamma> x)) \<and> map_of \<Gamma> x = map_of \<Gamma> y))))"
+
+lemma ind_for_heapVars_subset:
+  "ind_for is \<Gamma> \<Longrightarrow> heapVars is \<subseteq> heapVars \<Gamma>"
+  unfolding ind_for_def heapVars_def by auto
+
+lemma ind_var_or_lambda:
+  "ind_for is \<Gamma> \<Longrightarrow> x \<in> heapVars is \<Longrightarrow> isVar (the (map_of \<Gamma> x)) \<or> isLam ( the (map_of \<Gamma> x))"
+  unfolding heapVars_def ind_for_def by auto
+
+
+
+lemma map_of_from_set[simp]: "distinctVars \<Gamma> \<Longrightarrow> (x, e) \<in> set \<Gamma> \<Longrightarrow> map_of \<Gamma> x = Some e" sorry
+lemma map_of_from_set_iff[simp]: "distinctVars \<Gamma> \<Longrightarrow> map_of \<Gamma> x = Some e \<longleftrightarrow> (x, e) \<in> set \<Gamma>" sorry
+
+lemma map_of_not_from_set[simp]: "x \<notin> heapVars \<Gamma> \<Longrightarrow> map_of \<Gamma> x = None" by (metis domIff dom_map_of_conv_heapVars)
+
+lemma map_of_not_from_set_iff[simp]: "map_of \<Gamma> x = None \<longleftrightarrow> x \<notin> heapVars \<Gamma>" by (metis domIff dom_map_of_conv_heapVars)
+
+
+lemma ind_var_or_lambda2:
+  "distinctVars \<Gamma> \<Longrightarrow> ind_for is \<Gamma> \<Longrightarrow> (x,e) \<in> set \<Gamma> \<Longrightarrow> x \<in> heapVars is \<Longrightarrow> isVar e \<or> isLam e"
+  by (auto dest: ind_var_or_lambda)
+
+lemma ind_for_Cons[simp]: "distinctVars ((x,e)#\<Gamma>) \<Longrightarrow> \<not> isVar e \<Longrightarrow> \<not> isLam e \<Longrightarrow> ind_for is ((x,e)#\<Gamma>) \<longleftrightarrow> ind_for is \<Gamma>"
+  unfolding ind_for_def
+  by (auto simp add: distinctVars_Cons)
+
+(*
 lemma ind_for_Cons_notHeapVar[simp]: "x \<notin> heapVars is \<Longrightarrow> ind_for is ((x,e)#\<Gamma>) \<longleftrightarrow> ind_for is \<Gamma>"
   unfolding ind_for_def heapVars_def by fastforce
+*)
 
-lemma ind_for_larger_set: "ind_for is \<Gamma> \<Longrightarrow> set \<Gamma>  \<subseteq> set \<Gamma>' \<Longrightarrow> ind_for is \<Gamma>'"
-  unfolding ind_for_def by fastforce
-
-lemma ind_for_larger[simp]: "ind_for is \<Gamma> \<Longrightarrow> ind_for is (x#\<Gamma>)"
-  by (auto elim: ind_for_larger_set)
+lemma ind_for_larger_set: "distinctVars \<Gamma>' \<Longrightarrow> distinctVars \<Gamma> \<Longrightarrow> ind_for is \<Gamma> \<Longrightarrow> set \<Gamma>  \<subseteq> set \<Gamma>' \<Longrightarrow> ind_for is \<Gamma>'"
+  unfolding ind_for_def
+  apply (auto dest!: bspec)
+  apply (auto simp add: heapVars_def)[3]
+  apply (subgoal_tac "y \<in> heapVars \<Gamma>")
+  sorry
   
-lemma ind_for_permutation: "ind_for is \<Gamma> \<Longrightarrow> \<Gamma> <~~> \<Gamma>' \<Longrightarrow> ind_for is \<Gamma>'"
-  by (auto elim: ind_for_larger_set simp add: perm_set_eq)
+lemma ind_for_larger[simp]: "distinctVars \<Gamma> \<Longrightarrow> x \<notin> heapVars \<Gamma> \<Longrightarrow> ind_for is \<Gamma> \<Longrightarrow> ind_for is ((x,y)#\<Gamma>)"
+  by (auto intro: ind_for_larger_set simp add: distinctVars_Cons)
+  
+lemma ind_for_permutation: "distinctVars \<Gamma> \<Longrightarrow> ind_for is \<Gamma> \<Longrightarrow> \<Gamma> <~~> \<Gamma>' \<Longrightarrow> ind_for is \<Gamma>'"
+  by (auto intro: ind_for_larger_set[where \<Gamma> = \<Gamma>] simp add: perm_set_eq perm_distinctVars)
 
-lemma ind_for_ConsCons[simp]: "ind_for is (\<Gamma>) \<Longrightarrow> ind_for ((x,y)#is) ((x,Var y)#\<Gamma>)"
+lemma ind_for_ConsCons[simp]: "x \<notin> heapVars \<Gamma> \<Longrightarrow> ind_for is \<Gamma> \<Longrightarrow> ind_for ((x,y)#is) ((x,Var y)#\<Gamma>)"
   unfolding ind_for_def by auto
-
-lemma ind_for_subset:  "ind_for is \<Gamma> \<Longrightarrow> heapVars is \<subseteq> heapVars \<Gamma>"
-  unfolding ind_for_def heapVars_def 
-  apply (auto dest: imageE dest!: bspec)
-  by (metis heapVars_def heapVars_from_set)
 
 lemma ind_for_supp_subset:
   assumes "ind_for is \<Gamma>"
   shows "supp is \<subseteq> supp \<Gamma>"
+sorry
+(*
 proof
   fix x 
   assume "x \<in> supp is"
@@ -82,6 +132,7 @@ proof
     by (auto simp add: supp_Pair exp_assn.supp)
   thus "x \<in> supp \<Gamma>" by (metis (full_types) set_mp supp_set_mem)
 qed
+*)
 
 lemma ind_for_fresh: "ind_for is \<Gamma> \<Longrightarrow> a \<sharp> \<Gamma> \<Longrightarrow> a \<sharp> is"
   by (auto dest: ind_for_supp_subset simp add: fresh_def)
@@ -130,8 +181,8 @@ qed
 
 lemma ind_for_induct[consumes 1, case_names NoInd Ind]:
   assumes "valid_ind is"
-  assumes NoInd: "\<And> x. x \<notin> heapVars is \<Longrightarrow> P x"
-  assumes Ind: "\<And> x y. P y \<Longrightarrow> (x,y) \<in> set is \<Longrightarrow> P x"
+  assumes NoInd: "\<And> x. valid_ind is \<Longrightarrow> x \<notin> heapVars is \<Longrightarrow> P x"
+  assumes Ind: "\<And> x y.  valid_ind is \<Longrightarrow> P y \<Longrightarrow> (x,y) \<in> set is \<Longrightarrow> P x"
   shows "P x"
 proof(cases "x \<in> heapVars is")
 case True
@@ -152,16 +203,58 @@ case True
       show ?thesis.
     next
     case False
-      thus ?thesis by (rule NoInd)
+      thus ?thesis by (rule NoInd[OF assms(1)])
     qed
     moreover
     from less have "(x,y) \<in> set is" by (metis nth_mem)
     ultimately
-    show ?case by (rule Ind)
+    show ?case by (rule Ind[OF assms(1)])
   qed
 next
 case False
-  thus ?thesis by (rule NoInd)
+  thus ?thesis by (rule NoInd[OF assms(1)])
+qed
+
+thm ind_for_induct
+
+lemma ind_for_isLam: "ind_for is \<Gamma> \<Longrightarrow> (x,y) \<in> set is \<Longrightarrow> isLam (the (map_of \<Gamma> x)) \<Longrightarrow> isLam (the (map_of \<Gamma> y))"
+  unfolding ind_for_def by auto
+
+lemma resolve_isLam_there: "valid_ind is \<Longrightarrow> ind_for is \<Gamma> \<Longrightarrow> x \<in> heapVars is \<Longrightarrow> (x \<ominus> is) \<in> heapVars \<Gamma>" 
+  apply (induct x rule:ind_for_induct)
+  apply simp
+  apply auto
+  apply (simp add: resolve_var_same_image)
+  apply (case_tac "y \<in> heapVars is")
+  apply auto
+  sorry
+
+lemma resolve_isLam_isLam: "valid_ind is \<Longrightarrow> ind_for is \<Gamma> \<Longrightarrow> x \<in> heapVars is \<Longrightarrow> isLam (the (map_of \<Gamma> x)) \<Longrightarrow> isLam (the (map_of \<Gamma> (x \<ominus> is)))"
+  apply (induct x rule:ind_for_induct)
+  apply simp
+  apply auto
+  apply (drule (2) ind_for_isLam)
+  apply (simp add: resolve_var_same_image)
+  apply (case_tac "y \<in> heapVars is")
+  apply auto
+  done
+
+lemma Lambda_AnywhereI:
+  assumes "x \<in> heapVars \<Gamma>"
+  assumes "isLam (the (map_of \<Gamma> x))"
+  shows "\<Gamma> \<Down>\<^sup>i\<^sup>u\<^bsub>x#S\<^esub> \<Gamma>"
+proof-
+  from `x \<in> heapVars \<Gamma>` `isLam (the (map_of \<Gamma> x))`
+  obtain e where "(x,e) \<in> set \<Gamma>" and "isLam e"
+    apply (auto simp add: heapVars_def)
+    by (metis map_of_is_SomeD the.simps weak_map_of_SomeI)
+  obtain z e' where "e = Lam [z]. e'" by (metis `isLam e` isLam.simps(1) isLam.simps(3) isLam.simps(4) isVar.cases)
+  obtain \<Gamma>' where perm: "(x,Lam [z]. e') # \<Gamma>' <~~> \<Gamma>"
+    by (metis `(x, e) \<in> set \<Gamma>` `e = Lam [z]. e'` perm_remove perm_sym)
+
+  have "(x,Lam [z]. e') # \<Gamma>' \<Down>\<^sup>i\<^sup>u\<^bsub>x#S\<^esub> (x,Lam [z]. e') # \<Gamma>'" by (rule Lambda)
+  thus ?thesis
+    by (rule Permute[OF perm perm])
 qed
 
 lemma value_not_var:
@@ -181,27 +274,45 @@ theorem
        \<and> valid_ind is'
        \<and> S \<ominus>\<^sub>S is' = S \<ominus>\<^sub>S is"
 proof (nominal_induct \<Gamma> "\<surd>" u S \<Delta> avoiding: "is" rule:distinct_reds.strong_induct )
-case (DLambda x y e \<Gamma>' \<Gamma> u "is")
-  from DLambda have "x \<notin> heapVars is"
-    by (auto simp add: distinctVars_Cons dest: set_mp[OF ind_for_subset])
-  moreover
-  (* We need to rename y to avoid is *)
-  obtain y' :: var where "atom y' \<sharp> (y, e, is)" by (rule obtain_fresh)
-  {
-    hence "atom y' \<sharp> e" and "atom y' \<sharp> y" and "atom y' \<sharp> is" by (simp_all add: fresh_Pair)
-    from this(1,2)
-    have "Lam [y]. e = Lam [y']. ((y \<leftrightarrow> y') \<bullet> e)"
-      by (rule change_Lam_Variable)
-    also
-    from `atom y' \<sharp> is`
-    have "(Lam [y']. ((y \<leftrightarrow> y') \<bullet> e)) \<ominus> is = Lam [y']. (((y \<leftrightarrow> y') \<bullet> e) \<ominus> is)"
-    by (rule resolveExp_Lam)
-    finally
-    have "(Lam [y]. e) \<ominus> is = Lam [y']. ((y \<leftrightarrow> y') \<bullet> e \<ominus> is)".
-  }
-  ultimately
-  show ?case using DLambda
-    by -(rule exI[where x = "is"], auto intro: reds.Lambda)
+case (DLambda x y e \<Gamma> S u "is")
+  show ?case
+  proof(cases "x \<in> heapVars is")
+  case True
+    hence [simp]: "x \<ominus> is \<noteq> x" by (rule resolve_var_modifies[OF `valid_ind _`, symmetric])
+
+    have "x \<ominus> is \<in> heapVars (\<Gamma> \<ominus>\<^sub>h is)" sorry
+    moreover
+    from resolve_isLam_isLam[OF  `valid_ind is` `ind_for is _` True]
+    have "isLam (the (map_of \<Gamma> (x \<ominus> is)))" by simp
+    hence "isLam (the (map_of (\<Gamma> \<ominus>\<^sub>h is) (x \<ominus> is)))" sorry
+    ultimately
+    have "\<Gamma> \<ominus>\<^sub>h is \<Down>\<^sup>\<times>\<^sup>u\<^bsub>(x \<ominus> is) # removeAll (x \<ominus> is) (S \<ominus>\<^sub>S is)\<^esub> \<Gamma> \<ominus>\<^sub>h is" by (rule Lambda_AnywhereI)
+    with `x \<in> heapVars is`
+    have "(x, Lam [y]. e) # \<Gamma> \<ominus>\<^sub>h is \<Down>\<^sup>\<times>\<^sup>u\<^bsub>x # S \<ominus>\<^sub>S is\<^esub> (x, Lam [y]. e) # \<Gamma> \<ominus>\<^sub>h is" by simp
+    with  `ind_for is ((x, Lam [y]. e) # \<Gamma>)`   `valid_ind is`
+    show ?thesis
+      by -(rule exI[where x = "is"], auto intro: reds.Lambda)
+  next
+  case False
+    moreover
+    (* We need to rename y to avoid is *)
+    obtain y' :: var where "atom y' \<sharp> (y, e, is)" by (rule obtain_fresh)
+    {
+      hence "atom y' \<sharp> e" and "atom y' \<sharp> y" and "atom y' \<sharp> is" by (simp_all add: fresh_Pair)
+      from this(1,2)
+      have "Lam [y]. e = Lam [y']. ((y \<leftrightarrow> y') \<bullet> e)"
+        by (rule change_Lam_Variable)
+      also
+      from `atom y' \<sharp> is`
+      have "(Lam [y']. ((y \<leftrightarrow> y') \<bullet> e)) \<ominus> is = Lam [y']. (((y \<leftrightarrow> y') \<bullet> e) \<ominus> is)"
+      by (rule resolveExp_Lam)
+      finally
+      have "(Lam [y]. e) \<ominus> is = Lam [y']. ((y \<leftrightarrow> y') \<bullet> e \<ominus> is)".
+    }
+    ultimately
+    show ?thesis using DLambda
+      by -(rule exI[where x = "is"], auto intro: reds.Lambda)
+  qed
 next
 case (DApplicationInd n \<Gamma> x e y S \<Delta> \<Theta> z e' u "is")
 
@@ -481,17 +592,19 @@ case (DVariable y x S \<Gamma> z \<Delta> "is")
     show ?thesis by blast
   qed
 next
-case (DVariableNoUpd y x S e \<Gamma> z \<Delta> "is")
-  from `distinctVars ((y, z) # (x, Var y) # \<Delta>)`
-  have "x \<noteq> y" by (auto simp add: distinctVars_Cons distinctVars_append)
+case (DVariableNoUpd n \<Gamma> x y e S \<Delta> z "is")
+  from `y \<notin> set (x # S)`
+  have "x \<noteq> y" by auto
 
-  from DVariableNoUpd(10)[OF  `ind_for is _` `valid_ind is`]
-  obtain is' where is': "(x, Var y) # (y, e) # \<Gamma> \<ominus>\<^sub>h is \<Down>\<^sup>\<times>\<^sup>\<times>\<^bsub>y # x # S \<ominus>\<^sub>S is\<^esub> (y, z) # (x, Var y) # \<Delta> \<ominus>\<^sub>h is'"
-    and "ind_for is' ((y, z) # (x, Var y) # \<Delta>)"
+  from `ind_for is ((x, Var y) # \<Gamma>)`
+  have "ind_for is ((n, e) # (x, Var y) # \<Gamma>)" by simp
+  from DVariableNoUpd(20)[OF this `valid_ind is`]
+  obtain is' where is': "(n, e) # (x, Var y) # \<Gamma> \<ominus>\<^sub>h is \<Down>\<^sup>\<times>\<^sup>\<times>\<^bsub>n # y # x # S \<ominus>\<^sub>S is\<^esub> (n, z) # (x, Var y) # \<Delta> \<ominus>\<^sub>h is'"
+    and "ind_for is' ((n, z) # (x, Var y) # \<Delta>)"
     and "heapVars is \<subseteq> heapVars is'"
     and "valid_ind is'"
-    and hV: " heapVars is' \<inter> heapVars ((x, Var y) # (y, e) # \<Gamma>) \<subseteq> heapVars is"
-    and "y # x # S \<ominus>\<^sub>S is' = y # x # S \<ominus>\<^sub>S is"
+    and hV: " heapVars is' \<inter> heapVars ((n, e) # (x, Var y) # \<Gamma>) \<subseteq> heapVars is"
+    and "n # y # x # S \<ominus>\<^sub>S is' = n # y # x # S \<ominus>\<^sub>S is"
     by blast
 
   show ?case
@@ -500,25 +613,29 @@ case (DVariableNoUpd y x S e \<Gamma> z \<Delta> "is")
     have "(x,y) \<in> set is"
     proof-
       from True obtain y' where "(x,y') \<in> set is" by (auto simp add: heapVars_def)
-      hence "(x, Var y') \<in> set  ((x, Var y) # (y, e) # \<Gamma>)"
-        using `ind_for is _`  by (auto simp add: ind_for_def dest:bspec)
-      with `distinctVars ((x, Var y) # (y, e) # \<Gamma>)`
+      hence "(x, Var y') \<in> set  ((x, Var y) # \<Gamma>)"
+        using `ind_for is ((x, Var y) # \<Gamma>)` by (auto simp add: ind_for_def dest:bspec)
+      with `distinctVars ((x, Var y) # \<Gamma>)`
       have "y' = y" by (metis Pair_inject distinctVars_ConsD(1) exp_assn.eq_iff(1) heapVars_from_set set_ConsD)
       with `_ \<in> set is` show ?thesis by simp
     qed
 
     have [simp]: "x \<ominus> is = y \<ominus> is" sorry
 
+    (*
     from `(x,y) \<in> set is`
     have [simp]: "y # x # S \<ominus>\<^sub>S is = x # S \<ominus>\<^sub>S is" by simp
+    *)
 
     from `x \<in> heapVars is` `heapVars is \<subseteq> heapVars is'`
     have "x \<in> heapVars is'" by auto
 
-    (* Here the variable is set back. How to show this? *)
-    have "(y, z) # \<Delta> \<ominus>\<^sub>h is' = (y, e) # \<Delta> \<ominus>\<^sub>h is'" sorry
-    with is' `x \<in> heapVars is` `x \<in> heapVars is'`
-    have "(x, Var y) # (y, e) # \<Gamma> \<ominus>\<^sub>h is \<Down>\<^sup>\<times>\<^sup>\<times>\<^bsub>x # S \<ominus>\<^sub>S is\<^esub> (y, e) # (x, z) # \<Delta> \<ominus>\<^sub>h is'" by simp
+    from `atom n \<sharp> is` have "n \<notin> heapVars is" by (metis heapVars_not_fresh)
+
+    from is' `x \<in> heapVars is` `x \<in> heapVars is'` `n \<notin> heapVars is`
+    have "(x, Var y) # \<Gamma> \<ominus>\<^sub>h is \<Down>\<^sup>\<times>\<^sup>\<times>\<^bsub>x # S \<ominus>\<^sub>S is\<^esub> (x, z) # \<Delta> \<ominus>\<^sub>h is'"
+      apply simp
+      sorry
     moreover
   
     from `ind_for is' _`
@@ -545,49 +662,47 @@ case (DVariableNoUpd y x S e \<Gamma> z \<Delta> "is")
     from `x \<notin> heapVars is` hV
     have "x \<notin> heapVars is'" by auto
 
-    from value_not_var[OF DVariableNoUpd(9), simplified] `ind_for is' _` `valid_ind is'`
-    have "y \<notin> heapVars is'"
-      by (metis DVariableNoUpd.hyps(3) distinctVars_ConsD(1) ind_for_Cons ind_for_heapVars_subset set_mp)
+    from value_not_var[OF DVariableNoUpd(19), simplified] `ind_for is' _` `valid_ind is'`
+    have "n \<notin> heapVars is'"
+      sorry
     with `heapVars is \<subseteq> heapVars is'`
-    have "y \<notin> heapVars is" by auto
+    have "n \<notin> heapVars is" by auto
 
     from `x \<notin> heapVars is` hV
     have "x \<notin> heapVars is'" by auto
 
     have [simp]: "e \<ominus> is' = e \<ominus> is" sorry
+    have [simp]: "y \<ominus> is' = y \<ominus> is" sorry
 
-    from `y \<notin> set (x # S)` `x \<noteq> y` `y \<notin> heapVars is`
-    have "y \<notin> set (x # (S \<ominus>\<^sub>S is))" by simp
+    have "atom n \<sharp> (\<Gamma> \<ominus>\<^sub>h is, x, y \<ominus> is, e \<ominus> is, S \<ominus>\<^sub>S is, \<Delta> \<ominus>\<^sub>h is', z \<ominus> is')" sorry
     moreover
-    from is' `y \<notin> heapVars is` `x \<notin> heapVars is` `y \<notin> heapVars is'` `x \<notin> heapVars is'`
-    have "(x, Var y) # (y, e \<ominus> is) # (\<Gamma> \<ominus>\<^sub>h is) \<Down>\<^sup>\<times>\<^sup>\<times>\<^bsub>y # x # (S \<ominus>\<^sub>S is)\<^esub> (y, z \<ominus> is') # (x, Var y) # (\<Delta> \<ominus>\<^sub>h is')"
+    from `y \<notin> set (x # S)` `x \<noteq> y` `n \<notin> heapVars is`
+    have "y \<ominus> is \<notin> set (x # (S \<ominus>\<^sub>S is))" sorry
+    moreover
+    have "(y \<ominus> is, e \<ominus> is) \<in> set (\<Gamma> \<ominus>\<^sub>h is)" sorry
+    moreover
+    from is' `n \<notin> heapVars is` `x \<notin> heapVars is` `n \<notin> heapVars is'` `x \<notin> heapVars is'`
+    have "(n, e \<ominus> is) # (x, Var (y \<ominus> is)) # (\<Gamma> \<ominus>\<^sub>h is) \<Down>\<^sup>\<times>\<^sup>\<times>\<^bsub>n # (y \<ominus> is) # x # (S \<ominus>\<^sub>S is)\<^esub> (n, z \<ominus> is') # (x, Var (y \<ominus> is)) # (\<Delta> \<ominus>\<^sub>h is')"
       by (simp add: resolveExp_Var)
     ultimately
-    have "(x, Var y) # (y, e \<ominus> is) # (\<Gamma> \<ominus>\<^sub>h is) \<Down>\<^sup>\<times>\<^sup>\<times>\<^bsub>x # (S \<ominus>\<^sub>S is)\<^esub> (y, e \<ominus> is) # (x, z \<ominus> is') # (\<Delta> \<ominus>\<^sub>h is')"
+    have "(x, Var (y \<ominus> is)) # (\<Gamma> \<ominus>\<^sub>h is) \<Down>\<^sup>\<times>\<^sup>\<times>\<^bsub>x # (S \<ominus>\<^sub>S is)\<^esub> (x, z \<ominus> is') # (\<Delta> \<ominus>\<^sub>h is')"
       by (rule VariableNoUpd)
-    hence "(x, Var y) # (y, e) # \<Gamma> \<ominus>\<^sub>h is \<Down>\<^sup>\<times>\<^sup>\<times>\<^bsub>x # S \<ominus>\<^sub>S is\<^esub> (y, e) # (x, z) # \<Delta> \<ominus>\<^sub>h is'"
-      using  `y \<notin> heapVars is` `x \<notin> heapVars is` `y \<notin> heapVars is'` `x \<notin> heapVars is'`
+    hence "(x, Var y) # \<Gamma> \<ominus>\<^sub>h is \<Down>\<^sup>\<times>\<^sup>\<times>\<^bsub>x # S \<ominus>\<^sub>S is\<^esub> (x, z) # \<Delta> \<ominus>\<^sub>h is'"
+      using  `n \<notin> heapVars is` `x \<notin> heapVars is` `n \<notin> heapVars is'` `x \<notin> heapVars is'`
       by (simp add: resolveExp_Var)
     moreover
   
     from `ind_for is' _` (* `y \<notin> heapVars is'` `x \<notin> heapVars is'` *)
-    have "ind_for is' ((x, Var y) # (y, z) # \<Delta>)"
-      apply (rule ind_for_permutation)
-      by (metis perm.swap)
-    with `x \<notin> heapVars is'`
-    have "ind_for is' ((x, z) # (y, z) # \<Delta>)"
-      by auto
-    hence "ind_for is' ((y, z) # (x, z) # \<Delta>)"
-      apply (rule ind_for_permutation)
-      by (metis perm.swap)
-    hence "ind_for is' ((y, e) # (x, z) # \<Delta>)"
+    have "ind_for is' ((x, z) # \<Delta>)"
       sorry
     moreover
     note `heapVars is \<subseteq> heapVars is'` `valid_ind is'`
     moreover
-    note hV
+    from hV
+    have "heapVars is' \<inter> heapVars ((x, Var y) # \<Gamma>) \<subseteq> heapVars is"
+      sorry
     moreover
-    from `y # x # S \<ominus>\<^sub>S is' = y # x # S \<ominus>\<^sub>S is`
+    from `n # y # x # S \<ominus>\<^sub>S is' = n # y # x # S \<ominus>\<^sub>S is`
     have "x # S \<ominus>\<^sub>S is' = x # S \<ominus>\<^sub>S is"
       sorry
     (*
